remove old apply type stuff

Cm/PiE/Eval.lean
@@ -3,21 +3,7 @@ import Cm.PiE.Ast
 open Expr
 
 /-
-Potential massive simplification:
-what is the point of apply?
-apply really should be handled by our rules, I think.
-I think we can simplify this significantly.
-
-Am I stupid? what is the point of apply?
-
-β x with apply = :: both (:: whatever apply)
-we can just do this with id.
-
-But then we get back to the question:
-how do we emualte the "combining" step in S x y z?
-
-(x z) (y z)?
-this is kind of just handled by the list. we'll see.
+apply just turns a list into an app.
 -/
 
 /-
@@ -25,6 +11,8 @@ For testing purposes.
 This mirrors is_step_once exactly.
 -/
 def do_step_apply : Expr → Except Error Expr
+  -- this apply rule allows treating a list as if it were a function application
+  | ::[::[apply _m _n, _α, _β], ::[f, x]] => pure <| f$ f x
   | ::[::[.id _o, _α], x] => pure x
   | e@::[::[(const _o _p), _α, _β], _c]
   | e@::[::[(const' _o _p), _α, _β], _c] => pure e
@@ -118,167 +106,6 @@ example : try_step_n 200 (f$ (f$ (f$ (quote?_n 3 (Ty 0)) (Ty 0)) (Ty 0)) (Ty 0))
 def imp? (α β : Expr) : Expr := ::[quote α, quote β]
 
 /-
-apply : ∀ (α : Type) (β : α → Type) (f : ∀ (x : α), β x) (x : α), β x
-
--/
-def apply.type_with_holes.mk_β (m n : Level) : Expr :=
-  -- with α in scope, β : α → Type
-  -- :: both (:: const (quote (quote Ty n)))
-  -- this const is wrong. α : Ty m, f := (const t_α ? α)
-  -- f looks fine ish.
-  -- missing a both. after α is applied, we should get
-  -- a future both that will pass along the (x : α)
-  both?₁
-    (α := (Ty m))
-    (f := (quote both?₀))
-    (g :=
-      both?₁
-        (α := (Ty m))
-        (f := (const?₁ (α := (Ty m)) (m := m.succ)))
-        (g := (quote <| quote <| Ty n))
-        (m := m.succ))
-   (m := m.succ)
-
-/-
-f : ∀ (x : α), β x
-this is originally with α and β in scope to make the type.
-first α, then β.
-:: both
-α assertion must be quoted twice to escape β arg
-and x binder within.
-
-f should be both'd such that it can accept the β binder
-x is also a binder, so it should e under a both as well.
-
-we can totally remove the apply part here.
-β x
-
-β = quote id
--/
-def apply.type_with_holes.mk_mk_f (m n : Level) : Expr :=
-  both?_n 3
-    (f := quote?_n₀ 2)
-    (g := quote id?)
-    (α := Ty m)
-
-example : try_step_n 500 (f$ (f$ (f$ (f$ (quote?_n₀ 3) (Ty 0)) (Ty 0)) (Ty 0)) (Ty 0)) = (.ok (Ty 0)) := rfl
-#eval try_step_n 1000 (f$ (apply.type_with_holes.mk_mk_f 1 3) (Ty 0))
-  >>= (fun e => try_step_n 1000 (f$ e (@id? (Ty 1) (.some 2))))
-
-def apply.type_with_holes (m n : Level) : Expr :=
-  -- with α in scope, β : α → Type
-  let mk_β : Expr := type_with_holes.mk_β m n
-
-  -- with α in scope, then β in scope
-  -- with α in scope, make :: both (:: (quote α) (quote (apply))
-  let mk_mk_f := type_with_holes.mk_mk_f m n
-
-  -- x : α. this will have α, then β, then f in scope, so we need to quote twice
-  -- :: both (:: (quote const) (:: both (:: (quote const) id)))
-  -- (:: both (:: (quote const) (:: both (:: (quote const) id)))) α = ::[const, ::[const, α]]
-  let mk_mk_x := quote?_n₀ 2
-
-  /-
-    out type = β x. this is apply ?0 ?0 t_β α β x
-    so, this only disregards f.
-    apply α β, then quote once
-    :: both (:: (quote both) (:: both (:: (quote (quote const)) (apply ?0 ?0 t_β))))
-    (:: both (:: (quote both) (:: both (:: (quote (quote const)) (apply ?0 ?0 t_β))))) α
-      = :: both (:: (quote const) (apply ?0 ?0 t_β α)
-    (:: both (:: (quote const) (apply ?0 ?0 t_β α)) β
-      = const (apply ?0 ?0 t_β α β)
-    (const (apply ?0 ?0 t_β α β)) f
-      = apply ?0 ?0 t_β α β
-    apply ?0 ?0 t_β α β x = β x
-  -/
-  let mk_mk_t_out := both?
-    (f := (quote both?₀))
-    (g := both?
-      (f := quote <| quote <| const?₀)
-      (g := .app (apply 0 0) ?))
-
-  both?
-    (f := (quote?₁
-      (α := (Ty m.succ))
-      (e := (Ty m))
-      (m := m.succ.succ))) -- first arg, (α : Ty m)
-    (g := (both?_n 1 -- we will be under β here
-      (α := Ty m)
-      (f := mk_β) -- make β : α → Ty n from α
-      (g := (both?_n 2 -- we will be under f here
-        (α := Ty m)
-        (f := mk_mk_f)
-        (g := (both?_n 3 -- we will e under x here
-          (α := Ty m)
-          (f := mk_mk_x)
-          (g := mk_mk_t_out)))))))
-
-/-
-β = (K' (Ty 2) (Ty 1) (Ty 1)) (Ty 1) = (Ty 1)
-β = ((K' (Ty 2) (Ty 1) (Ty 1)) (Ty 1) : (Ty 2))
-
-β just gives us back Ty 1.
-f = (::[id 2, Ty 1])
-x = Ty 0
-
-t_f = ∀ (x : Ty 0), β x
-
-This is bringing up the question again of extensionality for
-function types.
-
-::[::[::[const'.{[3, 0]}, Ty 2, _], Ty 0], ::[const'.{[0, 0]}, _, _], Ty 2]
-How do we compare this against something similar but slightly different?
-This looks like [(quote Ty 0), (quote Ty 2)]. This is fine. α =
-
-This looks potentially quite suspicious:
-::[(@$ 0 0 _ _ ::[::[::[const'.{[0, 0]}, _, _], both'.{[0, 0, 0]}, _, _, _],
-     ::[both'.{[0, 0, 0]}, _, _, _],
-     ::[::[both'.{[0, 0, 0]}, _, _, _],
-       ::[::[const'.{[0, 0]}, _, _], Ty 1],
-       ::[const'.{[0, 0]}, _, _],
-       f$ (f$ (apply.{[0, 0]}) (_))
-       (_)],
-     ::[::[const'.{[0, 0]}, _, _], ::[const'.{[0, 0]}, _, _], both'.{[0, 0, 0]}, _, _, _],
-     ::[::[const'.{[0, 0]}, _, _], both'.{[0, 0, 0]}, _, _, _],
-     ::[both'.{[0, 0, 0]}, _, _, _],
-     ::[::[const'.{[0, 0]}, _, _], ::[const'.{[0, 0]}, _, _], (@$ 0 0 _ _ id.{[2]} Ty 1)],
-     ::[both'.{[0, 0, 0]}, _, _, _],
-     ::[::[const'.{[0, 0]}, _, _], const'.{[0, 0]}, _, _],
-     (@$ 0 0 _ _ f$ (apply.{[0, 0]}) (_) Ty 1)] ::[::[const'.{[3, 2]}, Ty 2, Ty 1], Ty 1]),
-  id.{[2]},
-  Ty 1]
-
-this is upon applying f to (t_apply α β)
-f should essentailly be totally discarded, ngl.
--/
-
-def test_reduce_apply_type : Except Error Expr := do
-  let m := 1
-  let t_α := Ty m.succ
-  let α := Ty m
-  let β := mk_quote m.succ.succ m.succ t_α α α -- discard (x : α), return α
-  let f := ::[id m.succ, α]
-  let x := Ty 0
-  -- first argument to apply type is α, then β,
-  -- then β, then f, then x
-  let a₁ ← try_step_n 500 ($? (apply.type_with_holes 2 2) α)
-  dbg_trace Expr.head! a₁ == (Ty 2)
-  let a₂ ← try_step_n 500 ($? a₁.tail! β)
-  dbg_trace Expr.head! a₂ == ::[Ty 1, Ty 2]
-  let a₃ := try_step_n 500 ($? a₂.tail! f)
-  dbg_trace a₃
-  dbg_trace (← try_step_n 200 ($? f x)) == (Ty 0)
-  -- got this for β: ::[::[::[const'.{[3, 0]}, Ty 2, _], Ty 1], ::[const'.{[0, 0]}, _, _], Ty 2]
-  -- (quote (Ty 1)) → (quote Ty 2), so this is ∀ (x : (Ty 1)), (Ty 2).
-  -- this seems right. probably β x = Ty 1, Ty 1 : Ty 2. fine.
-  .tail! <$> try_step_n 500 ($? (apply.type_with_holes 2 2) α)
-    >>= (fun e => .tail! <$> try_step_n 500 ($? e β))
-    >>= (fun e => .tail! <$> try_step_n 500 ($? e f))
-    >>= (fun e => .tail! <$> try_step_n 500 ($? e x))
-
-#eval test_reduce_apply_type
-
-/-
 id : ∀ (α : Type), α → α
 -/
 def id.type_with_holes (m : Level) : Expr :=
@@ -294,8 +121,8 @@ def id.type_with_holes (m : Level) : Expr :=
         (m := m.succ)))
       (m := m.succ)))
 
-example : Expr.tail! <$> try_step_n 500 (@$ 0 0 ? ? (id.type_with_holes 0) (Ty 0))
-  >>= (fun (e : Expr) => try_step_n 500 ((mk$ 0 0 ? ?) e (Ty 100))) = (.ok (::[Ty 0, Ty 0])) := rfl
+example : Expr.tail! <$> try_step_n 500 (f$ (id.type_with_holes 0) (Ty 0))
+  >>= (fun (e : Expr) => try_step_n 500 (f$ e (Ty 100))) = (.ok (::[Ty 0, Ty 0])) := rfl
 
 /-
 Type inference for filling in holes in expr types.
